@prefix cc: <http://creativecommons.org/ns#> .
@prefix dc: <http://purl.org/dc/terms/> .
@prefix foaf: <http://xmlns.com/foaf/0.1/> .
@prefix mini: <http://minipaas.org/rdf/ontology#> .
@prefix owl: <http://www.w3.org/2002/07/owl#> .
@prefix rdf: <http://www.w3.org/1999/02/22-rdf-syntax-ns#> .
@prefix rdfs: <http://www.w3.org/2000/01/rdf-schema#> .
@prefix vann: <http://purl.org/vocab/vann/> .
@prefix xsd: <http://www.w3.org/2001/XMLSchema#> .

<http://minipaas.org/rdf/ontology#> a owl:Ontology ;
    dc:creator "Kuno Woudt <kuno@frob.nl>" ;
    dc:modified "2014-05-16" ;
    vann:preferredNamespacePrefix "mini" ;
    vann:preferredNamespaceUri "http://minipaas.org/rdf/ontology#" .

mini:Service a owl:Class ;
    rdfs:label "Minipaas service description"@en .

mini:storage a owl:DatatypeProperty ;
    rdfs:label "requires storage plugin"@en ;
    rdfs:comment "This property specifies which storage plugin(s) are required to run the Minipaas packaged service."@en .

mini:License a owl:Class ;
    rdfs:label "License"@en ;
    rdfs:comment "This is the license under which a creative work is made available."@en .
    rdfs:subClassOf dc:LicenseDocument .

mini:license a owl:ObjectProperty ;
    rdfs:label "has license"@en ;
    rdfs:subPropertyOf dc:license, cc:license ;
    rdfs:domain mini:Service ;
    rdfs:range mini:License .

mini:licenseIdentifier a owl:DatatypeProperty ;
    rdfs:label "License ID"@en ;
    rdfs:comment "This is the license identifier for a (typically copyright) license. It must be a license short name The license identifier must be a license short name as used by debian, See https://www.debian.org/doc/packaging-manuals/copyright-format/1.0/#license-short-name."@en ;
    rdfs:subPropertyOf dc:identifier ;
    rdfs:domain mini:License ;
    rdfs:range xsd:string .

